1) SoftBound interfaces w/o shadow-stack were moved to src/Parser/tvcases/softbound-nss 2) *.c/h @ src/Parser/tvcases is the SoftBound with shadow stack 3) the src/Parser/tvcases/compileall.sh recompiles all cases under tvcases, setpath needs to be 'source' first. 4) extended SBpass to support functions, src/SoftBound/test.sh runs all available cases, fixed some bugs along the development.   Unfixed problems:   a) vargs is not supported, but all cases in olden-ccured/spec95 need this feathure.   b) failed for mutual recursive types, t1 = {t2*}  t2 = {t1*}   These two features disallow all large examples...
git-svn-id: https://webdav.seas.upenn.edu/svn/sol/vol@2926 eef5ea85-cc2e-0410-bd84-0fae1f012da8

src/SoftBound/main.ml
@@ -1,5 +1,6 @@
 open Ssa_interpreter
 open Sb_db_trans
+open Sb_ds_trans
 open Printf
 open Llvm
 open Trace
@@ -15,16 +16,10 @@ let main in_filename =
   let coqim = Llvm2coq.translate_module !Globalstates.debug ist im in
   (if !Globalstates.debug then Coq_pretty_printer.travel_module coqim);
 
-  (match SBpass.trans_module coqim with
+  (match SB_ds_pass.trans_module coqim with
   | Some coqom -> 
-(*      Coq_pretty_printer.travel_module coqom;*)
+      (if !Globalstates.debug then Coq_pretty_printer.travel_module coqom);
       Coq2ll.travel_module coqom
-(*
-        let om = Coq2llvm2.translate_module coqom in
-        (* write the module to a file *)
-        if not (Llvm_bitwriter.write_bitcode_file om out_filename) then 
-          exit 1
-*)
   | None -> failwith "failed");
 
   SlotTracker.dispose ist;
