src/ssa/ssa_wf.v
@@ -1,0 +1,129 @@
+Add LoadPath "./ott".
+Add LoadPath "./monads".
+Add LoadPath "./compcert".
+Add LoadPath "../../../theory/metatheory_8.3".
+Add LoadPath "../".
+Require Import ssa_def.
+Require Import ssa_lib.
+Require Import ssa_static.
+Require Import List.
+Require Import Arith.
+Require Import tactics.
+Require Import monad.
+Require Import trace.
+Require Import Metatheory.
+Require Import genericvalues.
+Require Import assoclist.
+Require Import Values.
+Require Import Memory.
+Require Import Integers.
+Require Import Coqlib.
+Require Import targetdata.
+Require Import GraphBasics.Digraphs.
+
+Export LLVMwf.
+
+Fixpoint blocks_to_Vset (bs:blocks) : V_set :=
+match bs with
+| nil => V_empty
+| block_intro l _ _ _ :: bs' => V_union (V_single (index l)) (blocks_to_Vset bs')
+end.
+
+Fixpoint blocks_to_Aset (bs:blocks) : A_set :=
+match bs with
+| nil => A_empty
+| block_intro l0 _ _ (insn_br _ _ l1 l2) :: bs' => 
+    A_union (A_single (A_ends (index l0) (index l1)))
+      (A_union (A_single (A_ends (index l0) (index l2))) (blocks_to_Aset bs'))
+| block_intro l0 _ _ (insn_br_uncond _ l1) :: bs' => 
+    A_union (A_single (A_ends (index l0) (index l1))) (blocks_to_Aset bs')
+| block_intro l0 _ _ _ :: bs' => blocks_to_Aset bs'
+end.
+
+Lemma blocks_to_Vset_spec : forall (blocks5 : blocks) (l0 : l) 
+  (H4 : l0 `notin` dom (genLabel2Block_blocks blocks5)),
+  ~ blocks_to_Vset blocks5 (index l0).
+Proof.
+  intros.
+  induction blocks5; intro J.
+    inversion J.
+
+    destruct a. simpl in *.
+    inversion J; subst.
+      inversion H; subst.
+      fsetdec.
+
+      apply IHblocks5; try solve [auto | fsetdec].
+Qed.
+
+Lemma blocks_to_CFG_no_edges : forall InF S MI FI bs,
+  wf_blocks InF S MI FI bs ->
+  uniq (genLabel2Block_blocks bs) ->
+  exists cfg : Digraph (blocks_to_Vset bs) A_empty, True.
+Proof.
+  intros InF S MI FI bs Hwfbs Huniq. 
+  induction Hwfbs; simpl; intros.
+    exists D_empty. auto.
+    
+    destruct block5 as [l0 ? ? tmn].
+    inversion Huniq; subst.
+    apply IHHwfbs in H2.
+    destruct H2 as [cfg _].
+    assert (~ blocks_to_Vset blocks5 (index l0)) as J.
+      eapply blocks_to_Vset_spec; eauto.
+    destruct tmn;
+      apply D_vertex with (x:=index l0) in cfg; 
+        try solve [auto | exists cfg; auto].
+Qed.
+
+Lemma Included_union_right : forall U (E F C: U_set U), 
+  Included U (Union U E F) C ->
+  Included U F C.
+Proof.
+        unfold Included in |- *; intros.
+        apply H. apply In_right. trivial.
+Qed.
+
+Lemma Included_union_left : forall U (E F C: U_set U), 
+  Included U (Union U E F) C ->
+  Included U E C.
+Proof.
+        unfold Included in |- *; intros.
+        apply H. apply In_left. trivial.
+Qed.
+
+Lemma blocks_to_CFG : forall InF S MI FI bs Vs,
+  wf_blocks InF S MI FI bs ->
+  uniq (genLabel2Block_blocks bs) ->
+  V_included (blocks_to_Vset bs) Vs ->
+  Digraph Vs A_empty ->
+  exists cfg : Digraph Vs (blocks_to_Aset bs), True.
+Proof.
+  intros InF S MI FI bs Vs Hwfbs Huniq Hinc Hcfg. 
+  induction Hwfbs; simpl in *; intros.
+    exists Hcfg. auto.
+    
+    destruct block5 as [l0 ? ? tmn]; simpl in *.
+    inversion Huniq; subst.
+    assert (J:=Hinc).
+    apply Included_union_left in J.
+    apply Included_union_right in Hinc.
+    apply IHHwfbs in H2; auto.
+    destruct H2 as [cfg _].
+    destruct tmn.
+      exists cfg. auto.
+      exists cfg. auto.
+
+      apply D_arc with (x:=index l0)(y:=index l2) in cfg.
+        apply D_arc with (x:=index l0)(y:=index l1) in cfg.
+          exists cfg. auto.
+          unfold Included in J. apply J. unfold V_single. apply In_single.
+Admitted.
+
+(*****************************)
+(*
+*** Local Variables: ***
+*** coq-prog-name: "coqtop" ***
+*** coq-prog-args: ("-emacs-U" "-I" "~/SVN/sol/vol/src/ssa/monads" "-I" "~/SVN/sol/vol/src/ssa/ott" "-I" "~/SVN/sol/vol/src/ssa/compcert" "-I" "~/SVN/sol/theory/metatheory_8.3" "-I" "~/SVN/sol/vol/src/TV" "-I" "~/SVN/sol/vol/src/GraphBasics" "-impredicative-set") ***
+*** End: ***
+ *)
