src/SoftBound/test.sh
@@ -9,8 +9,18 @@ ML_CASES="addrof all bug1 bug2 cint2ptr fptr fptr2 fptr3 fptrret free funcargs
 MC_DIR=../Parser/tvcases/microbench/
 MC_CASES="array array2 array3 global_array linkedlist linkedlistloop
           reference_test struct_array"
+OC_DIR=../Parser/tvcases/olden-ccured/
+# bh: llvm cannot compile it.
+# power: TV isn't terminating.
+# perimeter tsp have 'switch' instructions that we do not support so far.
+# em3d: removed 'free', since Softbound is not sound with 'free'.
+OC_CASES="bisort em3d health mst treeadd"
+S95_DIR=../Parser/tvcases/spec95-ccured/
+# 099.go 130.li 132.ijpeg has 'switch'
+S95_CASES="129.compress/src"
 
 for name in $ML_CASES; do 
+  rm -rf ./test
   echo -e $name": \c" ; 
   llvm-as -f $ML_DIR$name"/test-linked.ll" -o input.bc
   $SB input.bc >& output.ll
@@ -19,9 +29,9 @@ for name in $ML_CASES; do
   llvm-ld -native -lm -lcrypt test-softbound.bc -o test
   ./test 50
   ./test 55
-  rm -rf ./test
 done;
 for name in $MC_CASES; do 
+  rm -rf ./test
   echo -e $name": \c" ; 
   llvm-as -f $MC_DIR$name"/test-linked.ll" -o input.bc
   $SB input.bc >& output.ll
@@ -30,7 +40,26 @@ for name in $MC_CASES; do
   llvm-ld -native -lm -lcrypt test-softbound.bc -o test
   ./test 50
   ./test 55
+done;
+for name in $OC_CASES; do 
   rm -rf ./test
+  echo -e $name": \c" ; 
+  llvm-as -f $OC_DIR$name"/test-linked.ll" -o input.bc 
+  $SB input.bc >& output.ll
+  llvm-as -f output.ll
+  llvm-link output.bc softbound.bc softbound-wrappers.bc > test-softbound.bc
+  llvm-ld -native -lm -lcrypt test-softbound.bc -o test
+  ./test
+done;
+for name in $S95_CASES; do 
+  rm -rf ./test
+  echo -e $name": \c" ; 
+  llvm-as -f $S95_DIR$name"/test-linked.ll" -o input.bc 
+  $SB input.bc >& output.ll
+  llvm-as -f output.ll
+  llvm-link output.bc softbound.bc softbound-wrappers.bc > test-softbound.bc
+  llvm-ld -native -lm -lcrypt test-softbound.bc -o test
+  ./test
 done
 
 
